Use Kleene non-det choice instead of oracle in exec_seq.
exec_seq now also accumulates all of the intermediary results of the
operations, which makes the result appear stronger (the previous version surely
implied something like this, but that may not have been obvious.)

src/Spec/Layer.v
@@ -30,10 +30,10 @@ Fixpoint compile Op C_Op `(impl: LayerImpl C_Op Op) T (p: proc Op T) : proc C_Op
   | Bind p p' => Bind (impl.(compile) p) (fun v => impl.(compile) (p' v))
   end.
 
-Fixpoint compile_seq Op C_Op `(impl: LayerImpl C_Op Op) T R (p: proc_seq Op T R) :
-  proc_seq C_Op T R :=
+Fixpoint compile_seq Op C_Op `(impl: LayerImpl C_Op Op) R (p: proc_seq Op R) :
+  proc_seq C_Op R :=
   match p with
-  | Seq_Ret v => Seq_Ret v
+  | Seq_Nil => Seq_Nil
   | Seq_Bind p p' c => Seq_Bind (impl.(compile) p)
                                 (fun v => impl.(compile_seq) (p' v))
                                 (fun r => impl.(compile_seq) (c r))
@@ -208,16 +208,25 @@ Section Layers.
         rew H.
   Qed.
 
-  Theorem compile_exec_seq_ok T R (p: a_proc_seq T R) (rec: a_proc R) s:
+  Theorem compile_exec_seq_ok R (p: a_proc_seq R) (rec: a_proc R):
     refines rf.(absr)
-                 (exec_seq c_sem (compile_seq p) (compile_rec rec) s)
-                 (exec_seq a_sem p rec s).
+                 (exec_seq c_sem (compile_seq p) (compile_rec rec))
+                 (exec_seq a_sem p rec).
   Proof.
-    unfold refines; revert s;
-    induction p; intros s; do 2 rewrite exec_seq_unfold; simpl; norm.
-    destruct s as [[] s]; rewrite <-bind_assoc.
-    - rew compile_rexec_ok; repeat rel_congruence; eauto.
-    - rew compile_exec_ok; repeat rel_congruence; eauto.
+    unfold refines.
+    induction p as [| ??? IH1 ? IH2]; do 2 rewrite exec_seq_unfold; simpl; [ norm |].
+    setoid_rewrite bind_dist_r. setoid_rewrite bind_dist_l.
+    eapply or_respects_impl.
+    - rewrite <-bind_assoc.
+      rew compile_exec_ok; repeat rel_congruence; eauto.
+      rewrite <-bind_assoc.
+      setoid_rewrite IH1.
+      norm.
+    - rewrite <-bind_assoc.
+      rew compile_rexec_ok; repeat rel_congruence; eauto.
+      rewrite <-bind_assoc.
+      setoid_rewrite IH2.
+      norm.
   Qed.
 
   Theorem compile_ok : forall T (p: a_proc T) R (rec: a_proc R),
@@ -278,9 +287,9 @@ Section Layers.
     - Right.
   Qed.
 
-  Theorem complete_exec_seq_ok : forall T R (p: a_proc_seq T R) (rec: a_proc R) s,
-      test c_initP;; inited <- c_exec rf.(impl).(init); ifInit inited (c_sem.(exec_seq) (compile_seq p) (compile_rec rec) s) --->
-           (any (T:=unit);; test a_initP;; v <- a_sem.(exec_seq) p rec s; any (T:=unit);; pure (Some v)) +
+  Theorem complete_exec_seq_ok : forall R (p: a_proc_seq R) (rec: a_proc R),
+      test c_initP;; inited <- c_exec rf.(impl).(init); ifInit inited (c_sem.(exec_seq) (compile_seq p) (compile_rec rec)) --->
+           (any (T:=unit);; test a_initP;; v <- a_sem.(exec_seq) p rec; any (T:=unit);; pure (Some v)) +
       (any (T:=unit);; pure None).
   Proof.
     intros.
@@ -300,22 +309,22 @@ Section Layers.
   Qed.
 
   (* State a version without test, with some defns unfolded *)
-  Theorem complete_exec_seq_ok_alt T R (p: a_proc_seq T R) (rec: a_proc R) s
-      (cs1 cs2: CState) (mv: option T):
+  Theorem complete_exec_seq_ok_alt R (p: a_proc_seq R) (rec: a_proc R)
+      (cs1 cs2: CState) (mv: option (list ExecResult)):
     c_initP cs1 ->
     (inited <- c_exec rf.(impl).(init);
      match inited with
      | InitFailed => pure None
      | Initialized =>
-       v <- c_sem.(exec_seq) (compile_seq p) (compile_rec rec) s; pure (Some v)
+       v <- c_sem.(exec_seq) (compile_seq p) (compile_rec rec); pure (Some v)
      end) cs1 cs2 mv ->
     match mv with
     | None => True
-    | Some v => exists as1 as2, a_initP as1 /\ (a_sem.(exec_seq) p rec s) as1 as2 v
+    | Some v => exists as1 as2, a_initP as1 /\ (a_sem.(exec_seq) p rec) as1 as2 v
     end.
   Proof.
     intros.
-    pose proof (complete_exec_seq_ok p rec s).
+    pose proof (complete_exec_seq_ok p rec).
     unfold ifInit in H1. edestruct (H1 cs1 cs2 mv).
     { exists tt, cs1. split; [firstorder|].
       destruct H0 as (i&cs1'&?&?).
